Capless/Term.lean
@@ -1,5 +1,6 @@
 import Capless.CaptureSet
 import Capless.Type
+import Capless.Basic
 namespace Capless
 
 inductive Term : Nat -> Nat -> Nat -> Type where
@@ -23,5 +24,69 @@ inductive Term.IsValue : Term n m k -> Prop where
 | clam : Term.IsValue (clam t)
 | boxed : Term.IsValue (boxed x)
 | pack : Term.IsValue (pack c x)
+
+def Term.rename (t : Term n m k) (f : FinFun n n') : Term n' m k :=
+  match t with
+  | Term.var x => Term.var (f x)
+  | Term.lam E t => Term.lam (E.rename f) (t.rename f.ext)
+  | Term.tlam S t => Term.tlam (S.rename f) (t.rename f)
+  | Term.clam t => Term.clam (t.rename f)
+  | Term.boxed x => Term.boxed (f x)
+  | Term.pack c x => Term.pack c (f x)
+  | Term.app x y => Term.app (f x) (f y)
+  | Term.tapp x X => Term.tapp (f x) X
+  | Term.capp x c => Term.capp (f x) c
+  | Term.letin t u => Term.letin (t.rename f) (u.rename f.ext)
+  | Term.bindt S t => Term.bindt (S.rename f) (t.rename f)
+  | Term.bindc c t => Term.bindc (c.rename f) (t.rename f)
+  | Term.unbox c x => Term.unbox (c.rename f) (f x)
+
+def Term.trename (t : Term n m k) (f : FinFun m m') : Term n m' k :=
+  match t with
+  | Term.var x => Term.var x
+  | Term.lam E t => Term.lam (E.trename f) (t.trename f)
+  | Term.tlam S t => Term.tlam (S.trename f) (t.trename f.ext)
+  | Term.clam t => Term.clam (t.trename f)
+  | Term.boxed x => Term.boxed x
+  | Term.pack c x => Term.pack c x
+  | Term.app x y => Term.app x y
+  | Term.tapp x X => Term.tapp x (f X)
+  | Term.capp x c => Term.capp x c
+  | Term.letin t u => Term.letin (t.trename f) (u.trename f)
+  | Term.bindt S t => Term.bindt (S.trename f) (t.trename f.ext)
+  | Term.bindc c t => Term.bindc c (t.trename f)
+  | Term.unbox c x => Term.unbox c x
+
+def Term.crename (t : Term n m k) (f : FinFun k k') : Term n m k' :=
+  match t with
+  | Term.var x => Term.var x
+  | Term.lam E t => Term.lam (E.crename f) (t.crename f)
+  | Term.tlam S t => Term.tlam (S.crename f) (t.crename f)
+  | Term.clam t => Term.clam (t.crename f.ext)
+  | Term.boxed x => Term.boxed x
+  | Term.pack c x => Term.pack (f c) x
+  | Term.app x y => Term.app x y
+  | Term.tapp x X => Term.tapp x X
+  | Term.capp x c => Term.capp x (f c)
+  | Term.letin t u => Term.letin (t.crename f) (u.crename f)
+  | Term.bindt S t => Term.bindt (S.crename f) (t.crename f)
+  | Term.bindc c t => Term.bindc (c.crename f) (t.crename f.ext)
+  | Term.unbox c x => Term.unbox (c.crename f) x
+
+theorem IsValue.rename_l' {t : Term n m k} {t0 : Term n' m k}
+  (he : t0 = t.rename f)
+  (hv : t0.IsValue) :
+  t.IsValue := by
+  cases hv
+  all_goals (cases t <;> simp [Term.rename] at he; try constructor)
+
+theorem IsValue.rename_l {t : Term n m k}
+  (hv : (t.rename f).IsValue) :
+  t.IsValue := IsValue.rename_l' rfl hv
+
+theorem IsValue.rename_r {t : Term n m k}
+  (hv : t.IsValue) :
+  (t.rename f).IsValue := by
+  cases hv <;> simp [Term.rename] <;> constructor
 
 end Capless
