Capless/Renaming/Term/Typing.lean
@@ -1,0 +1,234 @@
+import Capless.Typing
+import Capless.Renaming.Basic
+import Capless.Renaming.Term.Subtyping
+namespace Capless
+
+theorem DropBinderFree.rename
+  (h : DropBinderFree C1 C2) :
+  DropBinderFree (C1.rename f.ext) (C2.rename f) := by
+  cases h
+  rw [<- CaptureSet.weaken_rename]
+  constructor
+
+theorem DropBinder.rename
+  (h : DropBinder C1 C2) :
+  DropBinder (C1.rename f.ext) (C2.rename f) := by
+  cases h
+  case drop_free =>
+    constructor; apply DropBinderFree.rename; assumption
+  case drop =>
+    simp [CaptureSet.rename_union]
+    simp [CaptureSet.rename_singleton, FinFun.ext]
+    rw [<- CaptureSet.weaken_rename]
+    apply DropBinder.drop
+
+theorem DropCBinder.rename
+  (h : DropCBinder C1 C2) :
+  DropCBinder (C1.rename f) (C2.rename f) := by
+  cases h
+  rw [CaptureSet.cweaken_rename_comm]
+  constructor
+
+theorem SealedLet.term_rename_l
+  (h : SealedLet (t.rename f) C) :
+  SealedLet t C := by
+  cases h
+  case mk hv _ =>
+    constructor
+    apply IsValue.rename_l hv
+    trivial
+
+theorem SealedLet.capture_rename_l'
+  (he : C0 = C.rename (FinFun.ext f))
+  (h : SealedLet t C0) :
+  SealedLet t C := by
+  cases h
+  case mk hv hl =>
+    constructor <;> try assumption
+    apply CaptureSet.nonlocal_rename_l he hl
+
+theorem SealedLet.capture_rename_l
+  (h : SealedLet t (C.rename (FinFun.ext f))) :
+  SealedLet t C := by
+  apply SealedLet.capture_rename_l'
+  rfl; assumption
+
+theorem SealedLet.neg_rename
+  (h : ¬SealedLet t C2) :
+  ¬SealedLet (t.rename f) (C2.rename f.ext) := by
+  intro h0
+  apply h
+  cases h0
+  case mk hv hl =>
+    constructor
+    apply IsValue.rename_l hv
+    apply CaptureSet.nonlocal_rename_l rfl hl
+
+theorem SealedLet.rename
+  (h : SealedLet t C) :
+  SealedLet (t.rename f) (C.rename f.ext) := by
+  cases h
+  case mk hv hl =>
+    constructor
+    apply IsValue.rename_r hv
+    apply CaptureSet.nonlocal_rename_r hl
+
+theorem Captured.rename
+  {f : FinFun n n'}
+  (h : Captured t C) :
+  Captured (t.rename f) (C.rename f) := by
+  induction h generalizing n'
+  case var =>
+    simp [Term.rename, CaptureSet.rename_singleton]
+    constructor
+  case lam ih =>
+    simp [Term.rename]
+    constructor
+    apply ih
+    apply DropBinder.rename; assumption
+  case tlam ih =>
+    simp [Term.rename]
+    constructor
+    apply ih
+  case clam ih =>
+    simp [Term.rename]
+    constructor
+    apply ih
+    apply DropCBinder.rename; assumption
+  case boxed =>
+    simp [Term.rename]
+    constructor
+  case pack =>
+    simp [Term.rename]
+    constructor
+  case app =>
+    simp [Term.rename, CaptureSet.rename_union, CaptureSet.rename_singleton]
+    constructor
+  case tapp =>
+    simp [Term.rename, CaptureSet.rename_singleton]
+    constructor
+  case capp =>
+    simp [Term.rename, CaptureSet.rename_singleton]
+    constructor
+  case letin ih1 ih2 =>
+    simp [Term.rename, CaptureSet.rename_union]
+    constructor
+    apply ih1
+    apply ih2
+    apply SealedLet.neg_rename; assumption
+    apply DropBinder.rename; assumption
+  case letin_sealed ih1 ih2 =>
+    simp [Term.rename]
+    constructor
+    apply ih1
+    rw [CaptureSet.weaken_rename]
+    apply ih2
+    rw [CaptureSet.weaken_rename]
+    apply SealedLet.rename; assumption
+  case unbox =>
+    simp [Term.rename, CaptureSet.rename_union]
+    constructor
+
+theorem Typing.rename
+  {Γ : Context n m k} {Δ : Context n' m k}
+  (h : Typed Γ t E)
+  (ρ : VarMap Γ f Δ) :
+  Typed Δ (t.rename f) (E.rename f) := by
+  induction h generalizing n'
+  case var hb =>
+    simp [Term.rename]
+    apply Typed.var
+    apply ρ.map; trivial
+  case exists_elim ih =>
+    simp [EType.rename, CType.rename, CaptureSet.rename_singleton, SType.copen_rename_comm]
+    simp [Term.rename]
+    have ih := ih ρ
+    simp [Term.rename, EType.rename, CType.rename] at ih
+    apply Typed.exists_elim
+    exact ih
+    rename_i hbc _
+    have hbc1 := ρ.cmap _ _ hbc
+    simp [CaptureSet.rename_rsingleton] at hbc1
+    trivial
+  case pack ih =>
+    simp [Term.rename, EType.rename]
+    apply Typed.pack
+    have ih := ih ρ
+    simp [Term.rename, EType.rename] at ih
+    rw [CType.copen_rename_comm] at ih
+    exact ih
+  case sub hs ih =>
+    apply Typed.sub
+    apply ih; trivial
+    apply ESubtyp.rename <;> trivial
+  case abs hcv iht =>
+    simp [Term.rename, EType.rename, CType.rename, SType.rename]
+    apply Typed.abs
+    apply iht <;> try assumption
+    apply ρ.ext
+    have hcv1 := hcv.rename (f := f)
+    simp [Term.rename] at hcv1
+    trivial
+  case tabs hcv iht =>
+    simp [Term.rename, EType.rename, CType.rename, SType.rename]
+    apply Typed.tabs
+    apply iht <;> try assumption
+    apply ρ.text
+    have hcv1 := hcv.rename (f := f)
+    simp [Term.rename] at hcv1
+    trivial
+  case cabs hcv iht =>
+    simp [Term.rename, EType.rename, CType.rename, SType.rename]
+    apply Typed.cabs
+    apply iht <;> try assumption
+    apply ρ.cext
+    have hcv1 := hcv.rename (f := f)
+    simp [Term.rename] at hcv1
+    trivial
+  case app ih1 ih2 =>
+    simp [Term.rename]
+    simp [EType.rename_open]
+    apply Typed.app
+    have ih1 := ih1 ρ
+    simp [Term.rename, EType.rename, CType.rename, SType.rename] at ih1
+    exact ih1
+    have ih2 := ih2 ρ
+    simp [Term.rename] at ih2
+    exact ih2
+  case tapp ih =>
+    simp [Term.rename]
+    simp [EType.rename_topen]
+    apply Typed.tapp
+    have ih := ih ρ
+    simp [Term.rename, EType.rename, CType.rename, SType.rename] at ih
+    trivial
+  case capp ih =>
+    simp [Term.rename, EType.rename_copen]
+    apply Typed.capp
+    have ih := ih ρ
+    simp [Term.rename, EType.rename, CType.rename, SType.rename] at ih
+    trivial
+  case box ih =>
+    simp [Term.rename, EType.rename, CType.rename, SType.rename]
+    simp [CaptureSet.rename_empty]
+    apply Typed.box
+    have ih := ih ρ
+    simp [Term.rename, EType.rename] at ih
+    trivial
+  case unbox ih =>
+    simp [Term.rename, EType.rename, CType.rename]
+    apply Typed.unbox
+    have ih := ih ρ
+    simp [Term.rename, EType.rename, CType.rename, CaptureSet.rename_empty] at ih
+    simp [SType.rename, CType.rename] at ih
+    trivial
+  case letin ih1 ih2 =>
+    simp [Term.rename]
+    apply Typed.letin
+    have ih1 := ih1 ρ
+    exact ih1
+    have ih2 := ih2 (ρ.ext _)
+    rw [<- EType.weaken_rename] at ih2
+    trivial
+
+end Capless
